Make coq-comparse more extraction friendly
Using coq-comparse was implying extracting [nat]/[Z] definitions and
functions due to the presence of [length] inside the [Input]
typeclass.

We split [Input] into two typeclasses, where [Input] only contains the
[unpack] function, and a newly introduced [InputLaws] living in [Prop]
introducing [length].

theories/Combinators.v
@@ -19,25 +19,31 @@ Open Scope monad_scope.
         succeeds at least once.
       - [many p] never fails. *)
 
-Function many_aux (i t : Type) (I : Input i t) (α : Type) (p : parser i α) (S : StrictParser p)
-    (input : i) (acc : list α) {measure length input}
+Function many_aux
+    (i t : Type) (len : i -> nat) (I : Input i t)
+    (L : @InputLaws i t len I) (α : Type) (p : parser i α)
+    (S : StrictParser len p)
+    (input : i) (acc : list α) {measure len input}
   : list α * i :=
   match runStateT p input with
-  | inr (x, output) => many_aux i t I α p S output (x :: acc)
+  | inr (x, output) => many_aux i t len I L α p S output (x :: acc)
   | inl _ => (rev acc, input)
   end.
 
 Proof.
-  intros i t I a p S input acc res x output eqr equ.
+  intros i t len I L a p S input acc res x output eqr equ.
   now apply is_strict in equ.
 Defined.
 
-Arguments many_aux {_ _ _ _} _ [_] _ _.
+Arguments many_aux {_ _ _ _ _ _} _ [_] _ _.
+Extraction Implicit many_aux [x1].
 
-Definition many `{Input i t} {α} (p : parser i α) `{StrictParser i t α p} : parser i (list α) :=
+Definition many `{I : Input i t} {α} (p : parser i α) `{StrictParser i t α len p} : parser i (list α) :=
   mkStateT (fun (input : i) => inr (many_aux p input [])).
 
-Instance many_parser `(StrictParser i t α p) : Parser (many p).
+Extraction Implicit many [I len].
+
+Instance many_parser `(StrictParser i t α len p) : Parser len (many p).
 
 Proof.
   unfold many.
@@ -46,7 +52,7 @@ Proof.
   cbn in equ.
   inversion equ.
   functional induction (many_aux p input []).
-  + transitivity (length output0).
+  + transitivity (len output0).
     ++ eapply IHp0; eauto.
     ++ now apply is_parser in e.
   + now inversion equ.
@@ -61,8 +67,10 @@ Qed.
       - [some p] is a _strict_ parser.
       - [some p] fails if [p] does not suceed at least once. *)
 
-Definition some `{Input i t} {α} (p : parser i α) `{StrictParser i t α p} : parser i (list α) :=
+Definition some `{I : Input i t} {α} (p : parser i α) `{StrictParser i t α len p} : parser i (list α) :=
   cons <$> p <*> (many p).
+
+Extraction Implicit some [I len].
 
 (** ** <<alt>> *)
 
@@ -73,7 +81,7 @@ Definition some `{Input i t} {α} (p : parser i α) `{StrictParser i t α p} : p
         consumes the same input as [p] or [q] would if applied directly.
       - [p <|> q] fails if both [p] and [q] fail. *)
 
-Definition alt `{Input i t} {α} (p q : parser i α) : parser i α :=
+Definition alt {i α} (p q : parser i α) : parser i α :=
   mkStateT (fun input =>
               match runStateT p input with
               | inl _ => runStateT q input
@@ -82,8 +90,9 @@ Definition alt `{Input i t} {α} (p q : parser i α) : parser i α :=
 
 Infix "<|>" := alt (at level 50, left associativity) : parser_scope.
 
-Instance alt_Parser `(Input i t, !@Parser i t α _ p, !@Parser i t α _  q)
-  : @Parser i t α _ (alt p q).
+Instance alt_Parser
+   `(InputLaws i t len, ! @Parser i t α len _ _ p, ! @Parser i t α len _ _ q)
+  : @Parser i t α len _ _ (alt p q).
 
 Proof.
   unfold alt.
@@ -101,8 +110,9 @@ Proof.
     now apply is_parser in equ'.
 Qed.
 
-Instance alt_Strict `(Input i t, !@StrictParser i t α _ p, !@StrictParser i t α _  q)
-  : @StrictParser i t α _ (alt p q).
+Instance alt_Strict
+   `(InputLaws i t len, !@StrictParser i t α len _ _ p, !@StrictParser i t α len _ _ q)
+  : @StrictParser i t α len _ _ (alt p q).
 
 Proof.
   unfold alt.
@@ -126,8 +136,7 @@ Qed.
       - [optional p] is _strict_ if [p] is _strict_. It consumes the same [input] as [p] would if applied directly.
       - [optional p] never fails. *)
 
-
-Definition optional `{Input i t} {α} (p : parser i α) : parser i (option α) :=
+Definition optional {i α} (p : parser i α) : parser i (option α) :=
   (Some <$> p) <|> pure None.
 
 (** ** <<fail>> *)
@@ -135,7 +144,7 @@ Definition optional `{Input i t} {α} (p : parser i α) : parser i (option α) :
 Definition fail {i α} (msg : string) : parser i α :=
   mkStateT (fun s => inl [msg]).
 
-Instance fail_Parser `(Input i t) : Parser (@fail i α msg).
+Instance fail_Parser `(InputLaws i t len) : Parser len (@fail i α msg).
 
 Proof.
   constructor.
@@ -152,7 +161,7 @@ Definition read_token `{Input i t} : parser i t :=
   | None => fail "expected character, found end of input"
   end.
 
-Instance read_token_Strict : StrictParser (@read_token i t H).
+Instance read_token_Strict `(InputLaws i t len) : StrictParser len (@read_token i t _).
 
 Proof.
   constructor.
@@ -164,7 +173,7 @@ Proof.
     rewrite equ' in equ.
     cbn in equ.
     inversion equ; subst.
-    rewrite (unpack_length input output x equ').
+    rewrite (unpack_len (InputLaws := H0) input output x equ').
     auto.
   + intros equ'.
     now rewrite equ' in equ.
@@ -186,32 +195,36 @@ Definition token `{RelDec t eqv, I : Input i t} (a : t) : parser i t :=
 (** ** <<tag>> *)
 
 Function tag_aux (i t : Type) (eqv : t -> t -> Prop) (H : @RelDec t eqv)
-    (I : Input i t) (x : i) (input : i)
-    {measure length x}
+    (len : i -> nat)
+    (I : Input i t) (L : InputLaws i t len) (x : i) (input : i)
+    {measure len x}
   : error_stack + (unit * i) :=
   match unpack input, unpack x with
   | Some (c, rst), Some (c', rst') =>
     if rel_dec c c'
-    then tag_aux i t _ H I rst' rst
+    then tag_aux i t _ H len I L rst' rst
     else inl ["nop"%string]
   | _, None => inr (tt, input)
   | _, _ => inl ["nop"%string]
   end.
 
 Proof.
-  intros i t H' H I x input [x' input'] c' rst' equ1 equ2 [y rst] y' rst'' equ3 equ4 equ5.
+  intros i t H' H len I L x input [x' input'] c' rst' equ1 equ2 [y rst] y' rst'' equ3 equ4 equ5.
   inversion equ3; subst.
-  apply unpack_length in equ4.
+  apply unpack_len in equ4.
   rewrite equ4.
   auto with arith.
 Defined.
 
-Arguments tag_aux [_ _ _ _ _] _ _.
+Arguments tag_aux [_ _ _ _ _ _ _] _ _.
+Extraction Implicit tag_aux [x3].
 
-Definition tag `{RelDec t eqv, Input i t} (x : i) : parser i unit :=
+Definition tag `{RelDec t eqv, InputLaws i t len} (x : i) : parser i unit :=
   mkStateT (fun input => tag_aux x input).
 
-Instance tag_parser `(RelDec t eqv, Input i t) : Parser (tag x).
+Extraction Implicit tag [len].
+
+Instance tag_parser `(RelDec t eqv, InputLaws i t len) : Parser len (tag x).
 
 Proof.
   intros x.
@@ -220,10 +233,10 @@ Proof.
   unfold tag in equ.
   cbn in *.
   functional induction (tag_aux x input).
-  + transitivity (length rst).
+  + transitivity (len rst).
     ++ apply IHs.
        apply equ.
-    ++ apply unpack_length in e.
+    ++ apply unpack_len in e.
        rewrite e.
        auto with arith.
   + discriminate.
@@ -235,9 +248,11 @@ Qed.
 (** [tag' x] is a variant of [tag x] which returns [x] and not [tt]. This can be
     useful used in conjunction of [<|>]. *)
 
-Definition tag' `{RelDec t eqv, Input i t} (x : i) : parser i i :=
+Definition tag' `{RelDec t eqv, InputLaws i t len} (x : i) : parser i i :=
   tag x;;
   pure x.
+
+Extraction Implicit tag' [len].
 
 (** ** <<many_until>> *)
 
@@ -247,32 +262,37 @@ Definition tag' `{RelDec t eqv, Input i t} (x : i) : parser i i :=
       - [many_until p q] is a _strict_ parser if _q_ is strict.
       - [many_until p q] fails if [p] fails before [q] could suceed. *)
 
-Function many_until_aux (α β i t : Type) (I : Input i t)
-    (p : parser i α) (H : StrictParser p) (q : parser i β)
-    (input : i) (acc : list α) {measure length input}
+Function many_until_aux (α β i t : Type) (len : i -> nat) (I : Input i t)
+    (L : InputLaws i t len)
+    (p : parser i α) (H : StrictParser len p) (q : parser i β)
+    (input : i) (acc : list α) {measure len input}
   : error_stack + (list α * i) :=
   match runStateT q input with
   | inl _ => match runStateT p input with
              | inl _ => inl ["p failed before q could succeed"%string]
-             | inr (x, output) => many_until_aux α β i t I p H q output (x :: acc)
+             | inr (x, output) => many_until_aux α β i t len I L p H q output (x :: acc)
              end
   | inr (_, output) => inr (rev acc, output)
   end.
 
 Proof.
-  intros α b i t I p H q input acc e eque res x output equr equ.
+  intros α b i t len I L p H q input acc e eque res x output equr equ.
   now apply is_strict in equ.
 Defined.
 
-Arguments many_until_aux [_ _ _ _ _] _ [_] _ _ _.
+Arguments many_until_aux [_ _ _ _ _ _ _] _ [_] _ _ _.
+Extraction Implicit many_until_aux [x3].
 
-Definition many_until {α β} `{Input i t}
-    (p : parser i α) `{StrictParser i t α p} (q : parser i β)
+Definition many_until {α β} `{InputLaws i t len}
+    (p : parser i α) `{StrictParser i t α len p} (q : parser i β)
   : parser i (list α) :=
   mkStateT (fun input => many_until_aux p q input []).
 
-Instance many_until_parser `(Input i t, !StrictParser (p : parser i a), !Parser (q : parser i b))
-  : Parser (many_until p q).
+Extraction Implicit many_until [len].
+
+Instance many_until_parser
+   `(InputLaws i t len, !StrictParser len (p : parser i a), !Parser len (q : parser i b))
+  : Parser len (many_until p q).
 
 Proof.
   constructor.
@@ -285,15 +305,16 @@ Proof.
     ++ discriminate.
     ++ destruct p0 as [y output'].
        inversion equ; subst.
-       transitivity (length output0).
+       transitivity (len output0).
        +++ now apply IHs.
        +++ now apply is_parser in e0.
   + inversion equ; subst.
     now apply is_parser in e.
 Qed.
 
-Instance many_until_strict `(Input i t, !StrictParser (p : parser i α), !StrictParser (q : parser i β))
-  : StrictParser (many_until p q).
+Instance many_until_strict
+   `(InputLaws i t len, !StrictParser len (p : parser i α), !StrictParser len (q : parser i β))
+  : StrictParser len (many_until p q).
 
 Proof.
   constructor.
@@ -306,7 +327,7 @@ Proof.
     ++ discriminate.
     ++ destruct p0 as [y output'].
        inversion equ; subst.
-       transitivity (length output0).
+       transitivity (len output0).
        +++ now apply IHs.
        +++ now apply is_strict in e0.
   + inversion equ; subst.
@@ -323,17 +344,21 @@ Qed.
       - [some_until p q] fails [p] does not succeeds at least once, and if [p]
         fails before [q] could succeed. *)
 
-Definition some_until {α β} `{Input i t}
-    (p : parser i α) `{StrictParser i t α p} (q : parser i β)
+Definition some_until {α β} `{InputLaws i t len}
+    (p : parser i α) `{StrictParser i t α len p} (q : parser i β)
   : parser i (list α) :=
   cons <$> p <*> many_until p q.
 
+Extraction Implicit some_until [len].
+
 (** ** <<sep>> *)
 
-Definition sep {α β} `{Input i t} (p : parser i α)
-    (q : parser i β) `{!StrictParser q, !Parser p}
+Definition sep {α β} `{InputLaws i t len} (p : parser i α)
+    (q : parser i β) `{!StrictParser len q, !Parser len p}
   : parser i (list α) :=
   cons <$> p <*> many (q;; p).
+
+Extraction Implicit sep [len].
 
 (** ** <<eoi>> *)
 
@@ -341,10 +366,10 @@ Definition eoi `{Input i t} : parser i unit :=
   mkStateT (fun input =>
               match unpack input with
               | None => inr (tt, input)
-              | Some (c, _) => inl [("Expected end of input, found " ++ token_to_text c)%string]
+              | Some (c, _) => inl [("Expected end of input, found " ++ token_to_string c)%string]
               end).
 
-Instance eoi_Parser `(Input i t) : Parser (eoi (i := i)).
+Instance eoi_Parser `(InputLaws i t len) : Parser len (eoi (i := i)).
 
 Proof.
   constructor.
@@ -371,7 +396,7 @@ Definition peek {i α} (p : parser i α) : parser i α :=
               | inl x => inl x
               end).
 
-Instance peek_Parser `(Input i t) (a : Type) (p : parser i a) : Parser (peek p).
+Instance peek_Parser `(InputLaws i t len) (a : Type) (p : parser i a) : Parser len (peek p).
 
 Proof.
   constructor.
